Working on thingy things

SafeAccess.v
@@ -14,113 +14,113 @@ From Elo Require Import References.
 (* ------------------------------------------------------------------------- *)
 
 Inductive UnsafeAccess (m : mem) : tm -> addr -> Prop :=
-  | unsafe_access_mem : forall ad ad' T,
+  | uacc_mem : forall ad ad' T,
     ad <> ad' ->
     UnsafeAccess m m[ad'] ad ->
     UnsafeAccess m <{ &ad' :: T }> ad
 
-  | unsafe_access_ref : forall ad T,
+  | uacc_ref : forall ad T,
     UnsafeAccess m <{ &ad :: &T }> ad
 
-  | unsafe_access_new : forall T t ad,
+  | uacc_new : forall T t ad,
     UnsafeAccess m t ad ->
     UnsafeAccess m <{ new T t }> ad
 
-  | unsafe_access_load : forall t ad,
+  | uacc_load : forall t ad,
     UnsafeAccess m t ad ->
     UnsafeAccess m <{ *t }> ad
 
-  | unsafe_access_asg1 : forall t1 t2 ad,
+  | uacc_asg1 : forall t1 t2 ad,
     UnsafeAccess m t1 ad ->
     UnsafeAccess m <{ t1 = t2 }> ad
 
-  | unsafe_access_asg2 : forall t1 t2 ad,
+  | uacc_asg2 : forall t1 t2 ad,
     UnsafeAccess m t2 ad ->
     UnsafeAccess m <{ t1 = t2 }> ad
 
-  | unsafe_access_fun : forall x Tx t ad,
+  | uacc_fun : forall x Tx t ad,
     UnsafeAccess m t ad ->
     UnsafeAccess m <{ fn x Tx --> t }> ad
 
-  | unsafe_access_call1 : forall t1 t2 ad,
+  | uacc_call1 : forall t1 t2 ad,
     UnsafeAccess m t1 ad ->
     UnsafeAccess m <{ call t1 t2 }> ad
 
-  | unsafe_access_call2 : forall t1 t2 ad,
+  | uacc_call2 : forall t1 t2 ad,
     UnsafeAccess m t2 ad ->
     UnsafeAccess m <{ call t1 t2 }> ad
 
-  | unsafe_access_seq1 : forall t1 t2 ad,
+  | uacc_seq1 : forall t1 t2 ad,
     UnsafeAccess m t1 ad ->
     UnsafeAccess m <{ t1; t2 }> ad
 
-  | unsafe_access_seq2 : forall t1 t2 ad,
+  | uacc_seq2 : forall t1 t2 ad,
     UnsafeAccess m t2 ad ->
     UnsafeAccess m <{ t1; t2 }> ad
   .
 
 Inductive SafeAccess (m : mem) : tm -> addr -> Prop :=
-  | safe_access_mem : forall ad ad' T,
+  | sacc_mem : forall ad ad' T,
     ad <> ad' ->
     SafeAccess m m[ad'] ad ->
     SafeAccess m <{ &ad' :: T }> ad
 
-  | safe_access_ref : forall ad T,
+  | sacc_ref : forall ad T,
     SafeAccess m <{ &ad :: i&T }> ad
 
-  | safe_access_new : forall t ad T,
+  | sacc_new : forall t ad T,
     SafeAccess m t ad ->
     SafeAccess m <{ new T t }> ad
 
-  | safe_access_load : forall t ad,
+  | sacc_load : forall t ad,
     SafeAccess m t ad ->
     SafeAccess m <{ *t }> ad
 
-  | safe_access_asg : forall t1 t2 ad,
+  | sacc_asg : forall t1 t2 ad,
     SafeAccess m t1 ad ->
     SafeAccess m t2 ad ->
     SafeAccess m <{ t1 = t2 }> ad
 
-  | safe_access_asg1 : forall t1 t2 ad,
+  | sacc_asg1 : forall t1 t2 ad,
     SafeAccess m t1 ad ->
     ~ UnsafeAccess m t2 ad ->
     SafeAccess m <{ t1 = t2 }> ad
 
-  | safe_access_asg2 : forall t1 t2 ad,
+  | sacc_asg2 : forall t1 t2 ad,
     SafeAccess m t2 ad ->
     ~ UnsafeAccess m t1 ad ->
     SafeAccess m <{ t1 = t2 }> ad
 
-  | safe_access_fun : forall x Tx t ad,
+  | sacc_fun : forall x Tx t ad,
     SafeAccess m t ad ->
     SafeAccess m <{ fn x Tx --> t }> ad
 
-  | safe_access_call : forall t1 t2 ad,
+  | sacc_call : forall t1 t2 ad,
     SafeAccess m t1 ad ->
     SafeAccess m t2 ad ->
     SafeAccess m <{ call t1 t2 }> ad
 
-  | safe_access_call1 : forall t1 t2 ad,
+  | sacc_call1 : forall t1 t2 ad,
     SafeAccess m t1 ad ->
     ~ UnsafeAccess m t2 ad ->
     SafeAccess m <{ call t1 t2 }> ad
 
-  | safe_access_call2 : forall t1 t2 ad,
+  | sacc_call2 : forall t1 t2 ad,
     SafeAccess m t2 ad ->
     ~ UnsafeAccess m t1 ad ->
     SafeAccess m <{ call t1 t2 }> ad
 
-  | safe_access_seq : forall t1 t2 ad,
+  | sacc_seq : forall t1 t2 ad,
     SafeAccess m t1 ad ->
     SafeAccess m t2 ad ->
     SafeAccess m <{ t1; t2 }> ad
 
-  | safe_access_seq1 : forall t1 t2 ad,
+  | sacc_seq1 : forall t1 t2 ad,
     SafeAccess m t1 ad ->
     ~ UnsafeAccess m t2 ad ->
     SafeAccess m <{ t1; t2 }> ad
 
-  | safe_access_seq2 : forall t1 t2 ad,
+  | sacc_seq2 : forall t1 t2 ad,
     SafeAccess m t2 ad ->
     ~ UnsafeAccess m t1 ad ->
     SafeAccess m <{ t1; t2 }> ad
@@ -128,56 +128,58 @@ Inductive SafeAccess (m : mem) : tm -> addr -> Prop :=
 
 Ltac inversion_sacc :=
   match goal with
-  | H : SafeAccess _ <{ unit }> _ |- _ => inversion_subst_clear H
-  | H : SafeAccess _ (_ _)      _ |- _ => inversion_subst_clear H
-  | H : SafeAccess _ (_ _ _)    _ |- _ => inversion_subst_clear H
-  | H : SafeAccess _ (_ _ _ _)  _ |- _ => inversion_subst_clear H
+  | H : SafeAccess _ <{ unit         }> _ |- _ => inversion_subst_clear H
+  | H : SafeAccess _ <{ N _          }> _ |- _ => inversion_subst_clear H
+  | H : SafeAccess _ <{ & _ :: _     }> _ |- _ => inversion_subst_clear H
+  | H : SafeAccess _ <{ new _ _      }> _ |- _ => inversion_subst_clear H
+  | H : SafeAccess _ <{ * _          }> _ |- _ => inversion_subst_clear H
+  | H : SafeAccess _ <{ _ = _        }> _ |- _ => inversion_subst_clear H
+  | H : SafeAccess _ <{ var _        }> _ |- _ => inversion_subst_clear H
+  | H : SafeAccess _ <{ fn _ _ --> _ }> _ |- _ => inversion_subst_clear H
+  | H : SafeAccess _ <{ call _ _     }> _ |- _ => inversion_subst_clear H
+  | H : SafeAccess _ <{ _ ; _        }> _ |- _ => inversion_subst_clear H
+  | H : SafeAccess _ <{ spawn _      }> _ |- _ => inversion_subst_clear H
   end.
 
 Ltac inversion_uacc :=
   match goal with
-  | H : UnsafeAccess _ <{ unit }> _ |- _ => inversion_subst_clear H
-  | H : UnsafeAccess _ (_ _)      _ |- _ => inversion_subst_clear H
-  | H : UnsafeAccess _ (_ _ _)    _ |- _ => inversion_subst_clear H
-  | H : UnsafeAccess _ (_ _ _ _)  _ |- _ => inversion_subst_clear H
+  | H : UnsafeAccess _ <{ unit         }> _ |- _ => inversion_subst_clear H
+  | H : UnsafeAccess _ <{ N _          }> _ |- _ => inversion_subst_clear H
+  | H : UnsafeAccess _ <{ & _ :: _     }> _ |- _ => inversion_subst_clear H
+  | H : UnsafeAccess _ <{ new _ _      }> _ |- _ => inversion_subst_clear H
+  | H : UnsafeAccess _ <{ * _          }> _ |- _ => inversion_subst_clear H
+  | H : UnsafeAccess _ <{ _ = _        }> _ |- _ => inversion_subst_clear H
+  | H : UnsafeAccess _ <{ var _        }> _ |- _ => inversion_subst_clear H
+  | H : UnsafeAccess _ <{ fn _ _ --> _ }> _ |- _ => inversion_subst_clear H
+  | H : UnsafeAccess _ <{ call _ _     }> _ |- _ => inversion_subst_clear H
+  | H : UnsafeAccess _ <{ _ ; _        }> _ |- _ => inversion_subst_clear H
+  | H : UnsafeAccess _ <{ spawn _      }> _ |- _ => inversion_subst_clear H
   end.
 
 (* ------------------------------------------------------------------------- *)
 (* Properties                                                                *)
 (* ------------------------------------------------------------------------- *)
 
-Theorem safe_access_then_access : forall m t ad,
+Theorem sacc_then_access : forall m t ad,
   SafeAccess m t ad ->
   access m t ad.
 Proof.
   intros * H. induction H; eauto using access.
 Qed.
 
-Theorem unsafe_access_then_access : forall m t ad,
+Theorem uacc_then_access : forall m t ad,
   UnsafeAccess m t ad ->
   access m t ad.
 Proof.
   intros * H. induction H; eauto using access.
 Qed.
 
-Theorem safe_then_not_unsafe : forall m t ad,
-  SafeAccess m t ad ->
-  ~ UnsafeAccess m t ad.
-Proof.
-  intros * Hsacc Huacc. induction Hsacc; inversion Huacc; subst; eauto.
-Qed.
-
-Corollary unsafe_then_not_safe : forall m t ad,
+Theorem not_uacc_sacc : forall m t ad,
   UnsafeAccess m t ad ->
-  ~ SafeAccess m t ad.
+  SafeAccess m t ad ->
+  False.
 Proof.
-  intros * F ?. contradict F. eauto using safe_then_not_unsafe.
-Qed.
-
-Corollary not_safe_and_unsafe : forall m t ad,
-  ~ (UnsafeAccess m t ad /\ SafeAccess m t ad).
-Proof.
-  intros * [F ?]. contradict F. eauto using safe_then_not_unsafe.
+  intros * Huacc ?. induction Huacc; inversion_sacc; eauto.
 Qed.
 
 Local Lemma length_ad' : forall m ad ad',
@@ -191,7 +193,7 @@ Proof.
   rewrite (get_default TM_Unit) in Hacc; try lia; inversion Hacc.
 Qed.
 
-Theorem access_to_unsafe_access : forall Gamma m t ad T,
+Theorem access_to_uacc : forall Gamma m t ad T,
   Gamma |-- t is T ->
   well_typed_memory m ->
   access m t ad ->
@@ -220,7 +222,7 @@ Proof.
   Unshelve. all: intros F; destruct F; eauto using SafeAccess.
 Qed.
 
-Theorem access_to_safe_access : forall Gamma m t ad T,
+Theorem access_to_sacc : forall Gamma m t ad T,
   Gamma |-- t is T ->
   well_typed_memory m ->
   access m t ad ->
@@ -243,16 +245,16 @@ Proof.
   Unshelve. all: intros F; destruct F; eauto using UnsafeAccess.
 Qed.
 
-Corollary safe_unsafe_dec : forall Gamma m t ad T,
+Corollary sacc_uacc_dec : forall Gamma m t ad T,
   well_typed_memory m ->
   Gamma |-- t is T ->
   access m t ad ->
   (SafeAccess m t ad \/ UnsafeAccess m t ad).
 Proof.
-  intros.
-  assert (decidable (UnsafeAccess m t ad))
-    as [? | ?]. { unfold decidable. eauto using excluded_middle. } (* TODO *)
+  intros. 
+  assert (decidable (UnsafeAccess m t ad)) as [? | ?] (* TODO *)
+      by eauto using classic_decidable.
   - right. assumption.
-  - left. eauto using access_to_safe_access.
+  - left. eauto using access_to_sacc.
 Qed.
 
